[IsaSAT] start defining state without tuple

Weidenbach_Book/IsaSAT/IsaSAT_Decide_LLVM.thy
@@ -10,18 +10,7 @@ sepref_def decide_lit_wl_fast_code
   unfolding decide_lit_wl_heur_def isasat_bounded_assn_def
   (*supply hn_case_prod'[sepref_comb_rules del]*)
   unfolding fold_tuple_optimizations
-  apply sepref_dbg_preproc
-  apply sepref_dbg_cons_init
-  apply sepref_dbg_id
-  apply sepref_dbg_monadify
-  apply sepref_dbg_opt_init
-  apply sepref_dbg_trans
-  apply sepref_dbg_opt
-  apply sepref_dbg_cons_solve
-  apply sepref_dbg_cons_solve
-  apply sepref_dbg_constraints
-  done
-
+  by sepref
 
 
 sepref_register find_unassigned_lit_wl_D_heur decide_lit_wl_heur
@@ -61,8 +50,261 @@ sepref_def find_unassigned_lit_wl_D_heur_impl
 sepref_def get_next_phase_st_impl
   is \<open>uncurry2 get_next_phase_st\<close>
   :: \<open>bool1_assn\<^sup>k *\<^sub>a atom_assn\<^sup>k *\<^sub>a isasat_bounded_assn\<^sup>k \<rightarrow>\<^sub>a bool1_assn\<close>
-  unfolding get_next_phase_st_def isasat_bounded_assn_def
+  unfolding get_next_phase_st_def isasat_bounded_assn_def fold_tuple_optimizations
   by sepref
+ML \<open>Sepref_Translate.gen_trans_step_tac\<close>
+thm sepref_fr_rules
+ML \<open>(Sepref_Translate.sepref_fr_rules.get @{context}) \<close>
+ML \<open>(Sepref_Translate.sepref_fr_rules.get @{context}) |> Tactic.build_net\<close>
+ML \<open>
+fun print start ctxt str _ = (print_tac ctxt (str ^ " " ^ (@{make_string} (Time.toMilliseconds (#elapsed (Timing.result start))))))
+
+    type phases_ctrl = {
+      trace: bool,            
+      trace_goals: bool,
+      int_res: bool,          
+      start: string option,   
+      stop: string option     
+    }
+    type phase = (unit -> string) * (Proof.context -> tactic') * int
+
+    local
+      fun ph_range (phases : phase list) start stop = let
+        fun find_phase name = let
+          val i = find_index (fn (n,_,_) => n()=name) phases
+          val _ = if i<0 then error ("No such phase: " ^ name) else ()
+        in
+          i
+        end
+
+        val i = case start of NONE => 0 | SOME n => find_phase n
+        val j = case stop of NONE => length phases - 1 | SOME n => find_phase n
+
+        val phases = take (j+1) phases |> drop i
+
+        val _ = case phases of [] => error "No phases selected, range is empty" | _ => ()
+      in
+        phases
+      end
+    in  
+  
+      fun PHASES' start phases (ctrl : phases_ctrl) ctxt = let
+        val phases = ph_range phases (#start ctrl) (#stop ctrl)
+        val phases = map (fn (n,tac,d) => (n,tac ctxt,d)) phases
+  
+        fun r [] _ st = Seq.single st
+          | r ((name,tac,d)::tacs) i st = let
+              val n = Thm.nprems_of st
+              val bailout_tac = if #int_res ctrl then all_tac else no_tac
+              fun trace_tac msg st = (if #trace ctrl then tracing msg else (); Seq.single st)
+              
+              val trace_goal_tac = if #trace_goals ctrl then print_tac ctxt "Proof state" else all_tac
+              
+              val trace_start_tac = trace_tac ("Phase " ^ (name ()))
+            in
+              K trace_goal_tac THEN' K trace_start_tac THEN' IF_EXGOAL (tac)
+              THEN_ELSE' (
+                fn i => fn st => 
+                  (* Bail out if a phase does not solve/create exactly the expected subgoals *)
+                  if Thm.nprems_of st = n+d then
+                    ((trace_tac ("  Done" ^ @{make_string} (Time.toMilliseconds (#elapsed (Timing.result start)))) THEN r tacs i) st)
+                  else
+                    (trace_tac "*** Wrong number of produced goals" THEN bailout_tac) st
+                
+              , 
+                K (trace_tac "*** Phase tactic failed" THEN bailout_tac))
+            end i st
+  
+      in
+        r phases
+      end
+
+
+    end
+
+
+    fun gen_trans_op_tac start dbg ctxt = let
+val _ = @{print} ("gen_trans_op_tac/start" ^ " " ^ 
+  (@{make_string} (Time.toMilliseconds (#elapsed (Timing.result start)))))
+      val fr_rl_net = Sepref_Translate.sepref_fr_rules.get ctxt |> Tactic.build_net
+      val fr_rl_tac = 
+        print start ctxt "fr_rl_tac/0" THEN'
+        resolve_from_net_tac ctxt fr_rl_net (* Try direct match *)
+        THEN' print start ctxt "fr_rl_tac/10"
+        ORELSE' (
+          Sepref_Frame.norm_goal_pre_tac ctxt (* Normalize precondition *) 
+        THEN' print start ctxt "fr_rl_tac/20"
+          THEN' (
+            resolve_from_net_tac ctxt fr_rl_net
+            THEN' print start ctxt "fr_rl_tac/30"
+            ORELSE' (
+              resolve_tac ctxt @{thms cons_pre_rule} (* Finally, generate a frame condition *)
+              THEN_ALL_NEW_LIST [
+                print start ctxt "fr_rl_tac/final/1" THEN'
+                SOLVED' (REPEAT_ALL_NEW_FWD (DETERM o resolve_tac ctxt @{thms CPR_TAG_rules})),
+                print start ctxt "fr_rl_tac/final/10" THEN'
+                K all_tac,  (* Frame remains unchanged as first goal, even if fr_rl creates side-conditions *)
+                print start ctxt "fr_rl_tac/final/20" THEN'
+                resolve_from_net_tac ctxt fr_rl_net
+              ]
+            )
+          )  
+        )
+      
+  (***** Side Condition Solving *)
+  local
+    open Sepref_Basic
+  in
+  
+    fun side_unfold_tac ctxt = let
+      (*val ctxt = put_simpset HOL_basic_ss ctxt
+        addsimps sepref_prep_side_simps.get ctxt*)
+    in
+      CONVERSION (Id_Op.unprotect_conv ctxt)
+      THEN' SELECT_GOAL (Local_Defs.unfold0_tac ctxt @{thms bind_ref_tag_def})
+      THEN' TRY o (hyp_subst_tac ctxt)
+      (*THEN' asm_full_simp_tac ctxt*)
+    end
+  
+    (* TODO: Not accessible as single ML function? *)
+    fun linarith_tac ctxt = 
+      Method.insert_tac ctxt (rev (Named_Theorems.get ctxt \<^named_theorems>\<open>arith\<close>))
+      THEN' Lin_Arith.tac ctxt
+    
+    fun bounds_tac ctxt = let
+      val ctxt = ctxt 
+        addSDs Named_Theorems_Rev.get ctxt @{named_theorems_rev sepref_bounds_dest}
+        addsimps Named_Theorems_Rev.get ctxt @{named_theorems_rev sepref_bounds_simps}
+    in
+      TRADE (fn ctxt => 
+        SELECT_GOAL (auto_tac ctxt)
+        THEN_ALL_NEW TRY o linarith_tac ctxt
+      ) ctxt
+    end
+    
+    fun side_fallback_tac ctxt = 
+      side_unfold_tac ctxt 
+      THEN' (
+print start ctxt "side_fallback_tac/auto" THEN'
+        TRADE (SELECT_GOAL o auto_tac) ctxt
+        THEN_ALL_NEW (print start ctxt "side_fallback_tac/auto/end" THEN' TRY o SOLVED' (bounds_tac ctxt))
+THEN' print start ctxt "side_fallback_tac/end"
+      )
+  
+    val side_frame_tac = Sepref_Frame.frame_tac side_fallback_tac
+    val side_merge_tac = Sepref_Frame.merge_tac side_fallback_tac
+    val side_free_tac = Sepref_Frame.free_tac side_fallback_tac
+    
+    
+    fun side_constraint_tac ctxt = Sepref_Constraints.constraint_tac ctxt
+    
+    val pf_mono_tac = Subgoal.FOCUS_PREMS (fn {context=ctxt,...} => CHANGED (ALLGOALS (Partial_Function.mono_tac ctxt)))
+    
+    fun side_mono_tac ctxt = side_unfold_tac ctxt THEN' TRADE pf_mono_tac ctxt
+  
+    fun side_gen_algo_tac ctxt = 
+      side_unfold_tac ctxt
+      THEN' resolve_tac ctxt (Named_Theorems_Rev.get ctxt @{named_theorems_rev sepref_gen_algo_rules})
+  
+    fun side_pref_def_tac ctxt = 
+      side_unfold_tac ctxt THEN' 
+      TRADE (fn ctxt => 
+        resolve_tac ctxt @{thms PREFER_tagI DEFER_tagI} 
+        THEN' (Sepref_Debugging.warning_tac' "Obsolete PREFER/DEFER side condition" ctxt THEN' Tagged_Solver.solve_tac ctxt)
+      ) ctxt
+
+
+    fun side_rprem_tac ctxt = 
+      resolve_tac ctxt @{thms RPREMI} THEN' Refine_Util.rprems_tac ctxt
+      THEN' (K (smash_new_rule ctxt))
+
+    (*
+      Solve side condition, or invoke hnr_tac on hn_refine goal.
+
+      In debug mode, side-condition solvers are allowed to not completely solve 
+      the side condition, but must change the goal.
+    *)  
+    fun side_cond_dispatch_tac start dbg hnr_tac ctxt = let
+      fun MK tac = if dbg then CHANGED o tac ctxt else SOLVED' (tac ctxt)
+
+      val t_merge = MK side_merge_tac
+      val t_frame = MK side_frame_tac
+      val t_free = MK side_free_tac
+      val t_indep = MK Indep_Vars.indep_tac
+      val t_constraint = MK side_constraint_tac
+      val t_mono = MK side_mono_tac
+      val t_pref_def = MK side_pref_def_tac
+      val t_rprem = MK side_rprem_tac
+      val t_gen_algo = side_gen_algo_tac ctxt
+      val t_cp_cond = MK (apply_method_noargs @{method cp_solve_cond})
+      val t_cp_simplify = MK (apply_method_noargs @{method cp_simplify})
+      
+      val t_fallback = MK side_fallback_tac
+      fun AROUND txt tac = print start ctxt ("start " ^ txt) THEN' tac THEN' print start ctxt ("end " ^ txt)
+    in
+      WITH_concl 
+        (fn @{mpat "Trueprop ?t"} => (case t of
+              @{mpat "MERGE _ _ _ _ _"} => AROUND "t_merge" t_merge
+            | @{mpat "MK_FREE _ _"} => AROUND "t_free" t_free
+            | @{mpat "_ \<turnstile> _"} => AROUND "t_frame" t_frame
+            | @{mpat "INDEP _"} => AROUND "indep" t_indep     (* TODO: Get rid of this!? *)
+            | @{mpat "CONSTRAINT _ _"} => AROUND "CONSTRAINT"  t_constraint
+            | @{mpat "M.mono_body _"} => AROUND "mono" t_mono
+            | @{mpat "PREFER_tag _"} => AROUND "pref" t_pref_def
+            | @{mpat "DEFER_tag _"} => AROUND "deref" t_pref_def
+            | @{mpat "RPREM _"} => AROUND "rprem" t_rprem
+            | @{mpat "GEN_ALGO _ _"} => AROUND "gen" t_gen_algo
+            | @{mpat "CP_cond _"} => AROUND "cond" t_cp_cond           
+            | @{mpat "CP_simplify _ _"} => AROUND "simplify" t_cp_simplify
+            | @{mpat "hn_refine _ _ _ _ _ _"} => AROUND "refine" hnr_tac 
+            | _ => AROUND "fallback" t_fallback
+          )
+        | _ => K no_tac  
+      )
+    end
+
+  end  
+      val side_tac = print start ctxt "side_tac/inner" THEN' REPEAT_ALL_NEW_FWD 
+(print start ctxt "side_tac/REPEAT_ALL_NEW_FWD" THEN' side_cond_dispatch_tac start false (K no_tac) ctxt)
+
+      val fr_tac = 
+ (*        if dbg then (* Present all possibilities with (partially resolved) side conditions *)
+          fr_rl_tac THEN_ALL_NEW_FWD (TRY o side_tac)
+        else (* Choose first rule that solves all side conditions *) *)
+          DETERM o SOLVED' (print start ctxt "fr_tac" THEN' fr_rl_tac THEN_ALL_NEW_FWD (print start ctxt "side_tac" THEN' SOLVED' side_tac))
+
+    in
+      PHASES' start [
+        (fn () => "Align goal" ^ " " ^ (@{make_string} (Time.toMilliseconds (#elapsed (Timing.result start)))),Sepref_Frame.align_goal_tac, 0),
+        (fn () => "Frame rule" ^ " " ^ (@{make_string} (Time.toMilliseconds (#elapsed (Timing.result start)))),fn ctxt => resolve_tac ctxt @{thms trans_frame_rule}, 1),
+        (* RECOVER_PURE goal *)
+        (fn () => "Recover pure" ^ " " ^ (@{make_string} (Time.toMilliseconds (#elapsed (Timing.result start)))),Sepref_Frame.recover_pure_tac, ~1),
+        (* hn-refine goal with stripped precondition *)
+        (fn () => "Apply rule" ^ " " ^ (@{make_string} (Time.toMilliseconds (#elapsed (Timing.result start)))),K fr_tac,~1)
+      ] (Sepref_Basic.flag_phases_ctrl ctxt dbg) ctxt
+    end
+
+      
+fun gen_trans_step_tac start dbg ctxt = Sepref_Translate.side_cond_dispatch_tac dbg
+      ( Sepref_Frame.norm_goal_pre_tac ctxt 
+        THEN' print start ctxt "THEN'"
+        THEN' ((print start ctxt "THEN'/1 start" 
+                 THEN' Sepref_Frame.align_goal_tac ctxt
+                 THEN' print start ctxt "THEN'/1 5"
+                 THEN' Sepref_Translate.trans_comb_tac ctxt THEN' print start ctxt "THEN'/1 end")
+              ORELSE' (print start ctxt "THEN'/2 start"
+                 THEN' gen_trans_op_tac start dbg ctxt THEN' print start ctxt "THEN'/2 end")))
+      ctxt\<close>
+setup \<open>map_theory_claset (fn ctxt => ctxt delSWrapper ("split_all_tac"))\<close>
+setup \<open>map_theory_claset (fn ctxt => ctxt addSbefore ("split_all_tac", split_all_tac))\<close>
+
+  method handle_CP_SEQ =  
+    drule CP_HANDLED,
+    erule CP_SEQE,
+    (elim conjE)?,
+    (*cp_sels_to_vars?,
+    cp_vars_to_sels?,*)
+    solves cp_resolve_tag | (cp_explode_prod?, cp_resolve_tag)
 
 sepref_def decide_wl_or_skip_D_fast_code
   is \<open>decide_wl_or_skip_D_heur\<close>
@@ -71,6 +313,100 @@ sepref_def decide_wl_or_skip_D_fast_code
   apply (rule hfref_refine_with_pre[OF decide_wl_or_skip_D_heur'_decide_wl_or_skip_D_heur, unfolded Down_id_eq])
   unfolding decide_wl_or_skip_D_heur'_def
   unfolding fold_tuple_optimizations option.case_eq_if atom.fold_option
+  apply sepref_dbg_preproc
+  apply sepref_dbg_cons_init
+  apply sepref_dbg_id
+  apply sepref_dbg_monadify
+  apply sepref_dbg_opt_init
+  apply sepref_dbg_trans_step
+  apply sepref_dbg_trans_step
+  apply sepref_dbg_trans_step
+  apply sepref_dbg_trans_step
+  apply sepref_dbg_trans_step
+  apply sepref_dbg_trans_step
+  apply sepref_dbg_trans_step
+  apply sepref_dbg_trans_step
+apply (tactic \<open> (REPEAT_DETERM_N 50 ( Sepref_Translate.trans_step_tac @{context} 1))\<close>)
+                      apply (tactic \<open> (REPEAT_DETERM_N 35 ( Sepref_Translate.trans_step_tac @{context} 1))\<close>)
+  supply [cp_solve_cond_pre] = CP_simps 
+  apply (rule CP_simplifyI)
+            apply (determ \<open>((thin_tac "_")+)?\<close>)
+            apply (rule impI)
+    apply ( (simp only: CP_simps cong: CP_tag_cong)?)
+            apply (determ \<open>cp_normalize_step\<close>)
+            apply (determ \<open>cp_normalize_step\<close>)
+               apply (determ \<open>cp_normalize_step\<close>)
+  apply (handle_CP_SEQ)
+  apply (drule CP_HANDLED,
+    erule CP_EXE)
+              apply ((elim conjE)?)
+  apply (subst (asm) prod_eq_iff)
+  apply (subst (asm) prod_eq_iff)
+  apply (subst (asm) prod_eq_iff)
+  apply (subst (asm) prod_eq_iff)
+  apply (subst (asm) prod_eq_iff)
+  apply (subst (asm) prod_eq_iff)
+  apply (subst (asm) prod_eq_iff)
+  apply (subst (asm) prod_eq_iff)
+  apply (subst (asm) prod_eq_iff)
+  apply (subst (asm) prod_eq_iff)
+  apply (subst (asm) prod_eq_iff)
+  apply (subst (asm) prod_eq_iff)
+  apply (subst (asm) prod_eq_iff)
+  apply (subst (asm) prod_eq_iff)
+  apply (subst (asm) prod_eq_iff)
+  apply (subst (asm) prod_eq_iff)
+  apply (subst (asm) prod_eq_iff)
+  apply (subst (asm) prod_eq_iff)
+  apply (subst (asm) prod_eq_iff)
+  apply (subst (asm) prod_eq_iff)
+  apply (subst (asm) prod_eq_iff)
+  apply (subst (asm) prod_eq_iff)
+  apply (subst (asm) prod_eq_iff)
+  apply (subst (asm) prod_eq_iff)
+  apply (subst (asm) prod_eq_iff)
+  apply (subst (asm) prod_eq_iff)
+  apply (subst (asm) prod_eq_iff)
+  apply (subst (asm) prod_eq_iff)
+  apply (subst (asm) prod_eq_iff)
+  apply (subst (asm) prod_eq_iff)
+  apply (subst (asm) prod_eq_iff)
+  apply (subst (asm) prod_eq_iff)
+  apply (subst (asm) prod_eq_iff)
+  apply (subst (asm) prod_eq_iff)
+  apply (subst (asm) prod_eq_iff)
+  apply (subst (asm) prod_eq_iff)
+  apply (subst (asm) prod_eq_iff)
+  apply (subst (asm) prod_eq_iff)
+              supply [[simp_trace=false]]
+               apply ((simp only: (* prod_eq_iff *)  prod.inject cnv_conj_to_meta (* fst_conv snd_conv *)  cong: CP_tag_cong))
+               apply (cp_resolve_tag)
+
+  thm prod_eq_iff
+              apply (drule CP_monos[THEN CP_HANDLEI] | handle_plain_eqs
+       |handle_CP_SEQ|handle_CP_EX(*handle_CP_EX32
+      |handle_CP_JOIN|handle_CP_RPT *)
+    
+)
+  unfolding CP_simps
+  apply (rule CP_simp_join_triv)
+  apply (tactic \<open>HEADGOAL (gen_trans_step_tac (Timing.start ()) true @{context})\<close>)
+apply (tactic \<open> (REPEAT_DETERM_N 50 ( Sepref_Translate.trans_step_tac @{context} 1))\<close>)
+  oops
+apply (tactic \<open> (REPEAT_DETERM_N 1 ( Sepref_Translate.trans_step_tac @{context} 1))\<close>)
+(*
+supply [[simp_trace]]
+apply sepref_dbg_trans_step
+  *)
+  oops
+apply (tactic \<open> (REPEAT_DETERM_N 1 ( Sepref_Translate.trans_step_tac @{context} 1))\<close>)
+oops
+  ML \<open>Sepref_Translate.trans_step_tac\<close>
+  apply sepref_dbg_opt
+  apply sepref_dbg_cons_solve
+  apply sepref_dbg_cons_solve
+  apply sepref_dbg_cons_solve_cp
+  apply sepref_dbg_constraints
   by sepref
 
 
