Weidenbach_Book/IsaSAT/IsaSAT_Setup0_LLVM.thy
@@ -7,12 +7,16 @@ theory IsaSAT_Setup0_LLVM
     IsaSAT_EMA_LLVM
     IsaSAT_Stats_LLVM
     IsaSAT_VDom_LLVM
+    Isabelle_LLVM.LLVM_DS_Block_Alloc
 begin
 
 no_notation WB_More_Refinement.fref (\<open>[_]\<^sub>f _ \<rightarrow> _\<close> [0,60,60] 60)
 no_notation WB_More_Refinement.freft (\<open>_ \<rightarrow>\<^sub>f _\<close> [60,60] 60)
-
-
+hide_const (open) NEMonad.ASSERT NEMonad.RETURN
+(* setup \<open>map_theory_claset (fn ctxt => ctxt delSWrapper ("split_all_tac"))\<close> *)
+term ll_bpto
+term ll_load
+  term ll_ref
 (*TODO Move*)
 
 paragraph \<open>Options\<close>
@@ -20,6 +24,552 @@ sepref_register mop_arena_length
 
 (* TODO: Move *)
 type_synonym arena_assn = \<open>(32 word, 64) array_list\<close>
+
+
+type_synonym twl_st_wll_trail_fast =
+  \<open>trail_pol_fast_assn \<times> arena_assn \<times> option_lookup_clause_assn \<times>
+    64 word \<times> watched_wl_uint32 \<times> vmtf_remove_assn \<times>
+    32 word \<times> cach_refinement_l_assn \<times> lbd_assn \<times> out_learned_assn \<times> stats \<times>
+    heur_assn \<times>
+   aivdom_assn \<times> (64 word \<times> 64 word \<times> 64 word \<times> 64 word \<times> 64 word) \<times>
+  opts_assn \<times> arena_assn\<close>
+
+
+(* datatype isasat_int = IsaSAT_int
+ *   (get_trail_wl_heur: trail_pol_fast_assn)
+ *   (get_clauses_wl_heur: arena_assn)
+ *   (get_conflict_wl_heur: option_lookup_clause_assn)
+ *   (literals_to_update_wl_heur: \<open>64 word\<close>)
+ *   (get_watched_wl_heur: \<open>watched_wl_uint32\<close>)
+ *   (get_vmtf_heur: vmtf_remove_assn)
+ *   (get_count_max_lvls_heur: \<open>32 word\<close>)
+ *   (get_conflict_cach: cach_refinement_l_assn)
+ *   (get_lbd: lbd_assn)
+ *   (get_outlearned_heur: out_learned_assn)
+ *   (get_heur: heur_assn)
+ *   (get_stats_heur: stats)
+ *   (get_aivdom: aivdom_assn)
+ *   (get_learned_count: \<open>64 word \<times> 64 word \<times> 64 word \<times> 64 word \<times> 64 word\<close>)
+ *   (get_opts: opts_assn)
+ *   (get_old_arena: arena_assn) *)
+
+datatype ('a, 'b, 'c, 'd, 'e, 'f, 'g, 'h, 'i, 'j, 'k, 'l, 'm, 'n, 'o, 'p) isasat_int = IsaSAT_int
+  (get_trail_wl_heur: 'a)
+  (get_clauses_wl_heur: 'b)
+  (get_conflict_wl_heur: 'c)
+  (literals_to_update_wl_heur: 'd)
+  (get_watched_wl_heur: 'e)
+  (get_vmtf_heur: 'f)
+  (get_count_max_lvls_heur: 'g)
+  (get_conflict_cach: 'h)
+  (get_lbd: 'i)
+  (get_outlearned_heur: 'j)
+  (get_heur: 'k)
+  (get_stats_heur: 'l)
+  (get_aivdom: 'm)
+  (get_learned_count: 'n)
+  (get_opts: 'o)
+  (get_old_arena: 'p)
+
+instantiation isasat_int ::
+  (llvm_rep,llvm_rep,llvm_rep,llvm_rep,
+  llvm_rep,llvm_rep,llvm_rep,llvm_rep,
+  llvm_rep,llvm_rep,llvm_rep,llvm_rep,
+  llvm_rep,llvm_rep,llvm_rep,llvm_rep) llvm_rep
+begin
+  definition to_val_isasat_int where
+    \<open>to_val_isasat_int \<equiv> (\<lambda>S. case S of
+     IsaSAT_int M N D i W ivmtf icount ccach lbd outl heur stats aivdom clss opts arena \<Rightarrow> LL_STRUCT [to_val M, to_val N, to_val D, to_val i, to_val W, to_val ivmtf,
+       to_val icount, to_val ccach, to_val lbd,
+       to_val outl, to_val heur, to_val stats, to_val aivdom,  to_val clss, to_val opts, to_val arena])\<close>
+
+  definition from_val_isasat_int :: \<open>llvm_val \<Rightarrow> ('a, 'b, 'c, 'd, 'e, 'f, 'g, 'h, 'i, 'j, 'k, 'l, 'm, 'n, 'o, 'p) isasat_int\<close> where
+    \<open>from_val_isasat_int \<equiv> (\<lambda>p. case llvm_val.the_fields p of
+   [M, N, D, i, W, ivmtf, icount, ccach, lbd, outl, heur, stats, aivdom, clss, opts, arena] \<Rightarrow>
+     IsaSAT_int (from_val M) (from_val N) (from_val D) (from_val i) (from_val W) (from_val ivmtf) (from_val icount) (from_val ccach) (from_val lbd)
+       (from_val outl) (from_val heur) (from_val stats) (from_val aivdom) (from_val clss) (from_val opts) (from_val arena))\<close>
+
+  definition [simp]: "struct_of_isasat_int (_ :: ('a, 'b, 'c, 'd, 'e, 'f, 'g, 'h, 'i, 'j, 'k, 'l, 'm, 'n, 'o, 'p) isasat_int itself) \<equiv>
+     VS_STRUCT [struct_of TYPE('a), struct_of TYPE('b), struct_of TYPE('c),
+      struct_of TYPE('d), struct_of TYPE('e), struct_of TYPE('f), struct_of TYPE('g), struct_of TYPE('h),
+      struct_of TYPE('i), struct_of TYPE('j), struct_of TYPE('k), struct_of TYPE('l),
+      struct_of TYPE('m), struct_of TYPE('n), struct_of TYPE('o), struct_of TYPE('p)]"
+
+  definition [simp]: "init_isasat_int :: ('a, 'b, 'c, 'd, 'e, 'f, 'g, 'h, 'i, 'j, 'k, 'l, 'm, 'n, 'o, 'p) isasat_int \<equiv> IsaSAT_int init init init init init init init init init init init init init init init init"
+
+  instance
+    apply standard
+    unfolding from_val_isasat_int_def to_val_isasat_int_def struct_of_isasat_int_def init_isasat_int_def comp_def isasat_int.case_distrib
+    subgoal
+      by (auto simp: init_zero fun_eq_iff from_val_isasat_int_def split: isasat_int.splits)
+    subgoal for v
+      by (cases v) (auto split: list.splits isasat_int.splits)
+    subgoal for v
+      by (cases v)
+       (simp add: LLVM_Shallow.null_def to_val_ptr_def split: isasat_int.splits)
+    subgoal
+      by (simp add: LLVM_Shallow.null_def to_val_ptr_def to_val_word_def init_zero split: isasat_int.splits)
+    done
+end
+subsubsection \<open>Setup for LLVM code export\<close>
+text \<open>Declare structure to code generator.\<close>
+lemma to_val_isasat_int[ll_to_val]: "to_val x = LL_STRUCT [
+  to_val (get_trail_wl_heur x),
+  to_val (get_clauses_wl_heur x),
+  to_val (get_conflict_wl_heur x),
+  to_val (literals_to_update_wl_heur x),
+  to_val (get_watched_wl_heur x),
+  to_val (get_vmtf_heur x),
+  to_val (get_count_max_lvls_heur x),
+  to_val (get_conflict_cach x),
+  to_val (get_lbd x),
+  to_val (get_outlearned_heur x),
+  to_val (get_heur x),
+  to_val (get_stats_heur x),
+  to_val (get_aivdom x),
+  to_val (get_learned_count x),
+  to_val (get_opts x),
+  to_val (get_old_arena x)]"
+  apply (cases x)
+  apply (auto simp: to_val_isasat_int_def)
+  done
+
+lemma node_insert_value:
+  "ll_insert_value (IsaSAT_int M N D i W ivmtf icount ccach lbd outl heur stats aivdom clss opts arena) M' 0 = Mreturn (IsaSAT_int M' N D i W ivmtf icount ccach lbd outl heur stats aivdom clss opts arena)"
+  "ll_insert_value (IsaSAT_int M N D i W ivmtf icount ccach lbd outl heur stats aivdom clss opts arena) N' (Suc 0) = Mreturn (IsaSAT_int M N' D i W ivmtf icount ccach lbd outl heur stats aivdom clss opts arena)"
+  "ll_insert_value (IsaSAT_int M N D i W ivmtf icount ccach lbd outl heur stats aivdom clss opts arena) D' 2 = Mreturn (IsaSAT_int M N D' i W ivmtf icount ccach lbd outl heur stats aivdom clss opts arena)"
+  "ll_insert_value (IsaSAT_int M N D i W ivmtf icount ccach lbd outl heur stats aivdom clss opts arena) i' 3 = Mreturn (IsaSAT_int M N D i' W ivmtf icount ccach lbd outl heur stats aivdom clss opts arena)"
+  "ll_insert_value (IsaSAT_int M N D i W ivmtf icount ccach lbd outl heur stats aivdom clss opts arena) W' 4 = Mreturn (IsaSAT_int M N D i W' ivmtf icount ccach lbd outl heur stats aivdom clss opts arena)"
+  "ll_insert_value (IsaSAT_int M N D i W ivmtf icount ccach lbd outl heur stats aivdom clss opts arena) ivmtf' 5 = Mreturn (IsaSAT_int M N D i W ivmtf' icount ccach lbd outl heur stats aivdom clss opts arena)"
+  "ll_insert_value (IsaSAT_int M N D i W ivmtf icount ccach lbd outl heur stats aivdom clss opts arena) icount' 6 = Mreturn (IsaSAT_int M N D i W ivmtf icount' ccach lbd outl heur stats aivdom clss opts arena)"
+  "ll_insert_value (IsaSAT_int M N D i W ivmtf icount ccach lbd outl heur stats aivdom clss opts arena) ccach' 7 = Mreturn (IsaSAT_int M N D i W ivmtf icount ccach' lbd outl heur stats aivdom clss opts arena)"
+  "ll_insert_value (IsaSAT_int M N D i W ivmtf icount ccach lbd outl heur stats aivdom clss opts arena) lbd' 8 = Mreturn (IsaSAT_int M N D i W ivmtf icount ccach lbd' outl heur stats aivdom clss opts arena)"
+  "ll_insert_value (IsaSAT_int M N D i W ivmtf icount ccach lbd outl heur stats aivdom clss opts arena) outl' 9 = Mreturn (IsaSAT_int M N D i W ivmtf icount ccach lbd outl' heur stats aivdom clss opts arena)"
+  "ll_insert_value (IsaSAT_int M N D i W ivmtf icount ccach lbd outl heur stats aivdom clss opts arena) heur' 10 = Mreturn (IsaSAT_int M N D i W ivmtf icount ccach lbd outl heur' stats aivdom clss opts arena)"
+  "ll_insert_value (IsaSAT_int M N D i W ivmtf icount ccach lbd outl heur stats aivdom clss opts arena) stats' 11 = Mreturn (IsaSAT_int M N D i W ivmtf icount ccach lbd outl heur stats' aivdom clss opts arena)"
+  "ll_insert_value (IsaSAT_int M N D i W ivmtf icount ccach lbd outl heur stats aivdom clss opts arena) aivdom' 12 = Mreturn (IsaSAT_int M N D i W ivmtf icount ccach lbd outl heur stats aivdom' clss opts arena)"
+  "ll_insert_value (IsaSAT_int M N D i W ivmtf icount ccach lbd outl heur stats aivdom clss opts arena) clss' 13 = Mreturn (IsaSAT_int M N D i W ivmtf icount ccach lbd outl heur stats aivdom clss' opts arena)"
+  "ll_insert_value (IsaSAT_int M N D i W ivmtf icount ccach lbd outl heur stats aivdom clss opts arena) opts' 14 = Mreturn (IsaSAT_int M N D i W ivmtf icount ccach lbd outl heur stats aivdom clss opts' arena)"
+  "ll_insert_value (IsaSAT_int M N D i W ivmtf icount ccach lbd outl heur stats aivdom clss opts arena) arena' 15 = Mreturn (IsaSAT_int M N D i W ivmtf icount ccach lbd outl heur stats aivdom clss opts arena')"
+  by (simp_all add: ll_insert_value_def llvm_insert_value_def Let_def checked_from_val_def
+                to_val_isasat_int_def from_val_isasat_int_def)
+
+lemma node_extract_value:
+  "ll_extract_value (IsaSAT_int M N D i W ivmtf icount ccach lbd outl heur stats aivdom clss opts arena) 0 = Mreturn M"
+  "ll_extract_value (IsaSAT_int M N D i W ivmtf icount ccach lbd outl heur stats aivdom clss opts arena) (Suc 0) = Mreturn N"
+  "ll_extract_value (IsaSAT_int M N D i W ivmtf icount ccach lbd outl heur stats aivdom clss opts arena) 2 = Mreturn D"
+  "ll_extract_value (IsaSAT_int M N D i W ivmtf icount ccach lbd outl heur stats aivdom clss opts arena) 3 = Mreturn i"
+  "ll_extract_value (IsaSAT_int M N D i W ivmtf icount ccach lbd outl heur stats aivdom clss opts arena) 4 = Mreturn W"
+  "ll_extract_value (IsaSAT_int M N D i W ivmtf icount ccach lbd outl heur stats aivdom clss opts arena) 5 = Mreturn ivmtf"
+  "ll_extract_value (IsaSAT_int M N D i W ivmtf icount ccach lbd outl heur stats aivdom clss opts arena) 6 = Mreturn icount"
+  "ll_extract_value (IsaSAT_int M N D i W ivmtf icount ccach lbd outl heur stats aivdom clss opts arena) 7 = Mreturn ccach"
+  "ll_extract_value (IsaSAT_int M N D i W ivmtf icount ccach lbd outl heur stats aivdom clss opts arena) 8 = Mreturn lbd"
+  "ll_extract_value (IsaSAT_int M N D i W ivmtf icount ccach lbd outl heur stats aivdom clss opts arena) 9 = Mreturn outl"
+  "ll_extract_value (IsaSAT_int M N D i W ivmtf icount ccach lbd outl heur stats aivdom clss opts arena) 10 = Mreturn heur"
+  "ll_extract_value (IsaSAT_int M N D i W ivmtf icount ccach lbd outl heur stats aivdom clss opts arena) 11 = Mreturn stats"
+  "ll_extract_value (IsaSAT_int M N D i W ivmtf icount ccach lbd outl heur stats aivdom clss opts arena) 12 = Mreturn aivdom"
+  "ll_extract_value (IsaSAT_int M N D i W ivmtf icount ccach lbd outl heur stats aivdom clss opts arena) 13 = Mreturn clss"
+  "ll_extract_value (IsaSAT_int M N D i W ivmtf icount ccach lbd outl heur stats aivdom clss opts arena) 14 = Mreturn opts"
+  "ll_extract_value (IsaSAT_int M N D i W ivmtf icount ccach lbd outl heur stats aivdom clss opts arena) 15 = Mreturn arena"
+  apply (simp_all add: ll_extract_value_def llvm_extract_value_def Let_def checked_from_val_def
+                to_val_isasat_int_def from_val_isasat_int_def)
+  done
+
+text \<open>Lemmas to translate node construction and destruction\<close>
+lemma inline_return_node[llvm_pre_simp]: "Mreturn (IsaSAT_int M N D i W ivmtf icount ccach lbd outl heur stats aivdom clss opts arena) = doM {
+    r \<leftarrow> ll_insert_value init M 0;
+    r \<leftarrow> ll_insert_value r N 1;
+    r \<leftarrow> ll_insert_value r D 2;
+    r \<leftarrow> ll_insert_value r i 3;
+    r \<leftarrow> ll_insert_value r W 4;
+    r \<leftarrow> ll_insert_value r ivmtf 5;
+    r \<leftarrow> ll_insert_value r icount 6;
+    r \<leftarrow> ll_insert_value r ccach 7;
+    r \<leftarrow> ll_insert_value r lbd 8;
+    r \<leftarrow> ll_insert_value r outl 9;
+    r \<leftarrow> ll_insert_value r heur 10;
+    r \<leftarrow> ll_insert_value r stats 11;
+    r \<leftarrow> ll_insert_value r aivdom 12;
+    r \<leftarrow> ll_insert_value r clss 13;
+    r \<leftarrow> ll_insert_value r opts 14;
+    r \<leftarrow> ll_insert_value r arena 15;
+    Mreturn r
+  }"
+  apply (auto simp: node_insert_value)
+  done
+
+lemma inline_node_case[llvm_pre_simp]: "(case r of (IsaSAT_int M N D i W ivmtf icount ccach lbd outl heur stats aivdom clss opts arena) \<Rightarrow> f M N D i W ivmtf icount ccach lbd outl heur stats aivdom clss opts arena) = doM {
+    M \<leftarrow> ll_extract_value r 0;
+    N \<leftarrow> ll_extract_value r 1;
+    D \<leftarrow> ll_extract_value r 2;
+    i \<leftarrow> ll_extract_value r 3;
+    W \<leftarrow> ll_extract_value r 4;
+    ivmtf \<leftarrow> ll_extract_value r 5;
+    icount \<leftarrow> ll_extract_value r 6;
+    ccach \<leftarrow> ll_extract_value r 7;
+    lbd \<leftarrow> ll_extract_value r 8;
+    outl \<leftarrow> ll_extract_value r 9;
+    heur \<leftarrow> ll_extract_value r 10;
+    stats \<leftarrow> ll_extract_value r 11;
+    aivdom \<leftarrow> ll_extract_value r 12;
+    clss \<leftarrow> ll_extract_value r 13;
+    opts \<leftarrow> ll_extract_value r 14;
+    arena \<leftarrow> ll_extract_value r 15;
+  f M N D i W ivmtf icount ccach lbd outl heur stats aivdom clss opts arena
+}"
+  apply (cases r)
+  apply (auto simp: node_extract_value)
+  done
+
+lemma inline_return_node_case[llvm_pre_simp]: "doM {Mreturn (case r of (IsaSAT_int M N D i W ivmtf icount ccach lbd outl heur stats aivdom clss opts arena) \<Rightarrow> f M N D i W ivmtf icount ccach lbd outl heur stats aivdom clss opts arena)} = doM {
+    M \<leftarrow> ll_extract_value r 0;
+    N \<leftarrow> ll_extract_value r 1;
+    D \<leftarrow> ll_extract_value r 2;
+    i \<leftarrow> ll_extract_value r 3;
+    W \<leftarrow> ll_extract_value r 4;
+    ivmtf \<leftarrow> ll_extract_value r 5;
+    icount \<leftarrow> ll_extract_value r 6;
+    ccach \<leftarrow> ll_extract_value r 7;
+    lbd \<leftarrow> ll_extract_value r 8;
+    outl \<leftarrow> ll_extract_value r 9;
+    heur \<leftarrow> ll_extract_value r 10;
+    stats \<leftarrow> ll_extract_value r 11;
+    aivdom \<leftarrow> ll_extract_value r 12;
+    clss \<leftarrow> ll_extract_value r 13;
+    opts \<leftarrow> ll_extract_value r 14;
+    arena \<leftarrow> ll_extract_value r 15;
+  Mreturn (f M N D i W ivmtf icount ccach lbd outl heur stats aivdom clss opts arena)
+}"
+  apply (cases r)
+  apply (auto simp: node_extract_value)
+  done
+
+lemmas [llvm_inline] =
+  isasat_int.get_trail_wl_heur_def
+  isasat_int.get_clauses_wl_heur_def
+  isasat_int.get_conflict_wl_heur_def
+  isasat_int.literals_to_update_wl_heur_def
+  isasat_int.get_watched_wl_heur_def
+  isasat_int.get_vmtf_heur_def
+  isasat_int.get_count_max_lvls_heur_def
+  isasat_int.get_conflict_cach_def
+  isasat_int.get_lbd_def
+  isasat_int.get_outlearned_heur_def
+  isasat_int.get_heur_def
+  isasat_int.get_stats_heur_def
+  isasat_int.get_aivdom_def
+  isasat_int.get_learned_count_def
+  isasat_int.get_opts_def
+  isasat_int.get_old_arena_def
+
+  term from_val
+  term uint64_nat_assn
+  term ll_bpto
+fun isasat_int_assn :: \<open>
+  ('a \<Rightarrow> _ \<Rightarrow> llvm_amemory \<Rightarrow> bool) \<Rightarrow>
+  ('b \<Rightarrow> _ \<Rightarrow> llvm_amemory \<Rightarrow> bool) \<Rightarrow>
+  ('c \<Rightarrow> _ \<Rightarrow> llvm_amemory \<Rightarrow> bool) \<Rightarrow>
+  ('d \<Rightarrow> _ \<Rightarrow> llvm_amemory \<Rightarrow> bool) \<Rightarrow>
+  ('e \<Rightarrow> _ \<Rightarrow> llvm_amemory \<Rightarrow> bool) \<Rightarrow>
+  ('f \<Rightarrow> _ \<Rightarrow> llvm_amemory \<Rightarrow> bool) \<Rightarrow>
+  ('g \<Rightarrow> _ \<Rightarrow> llvm_amemory \<Rightarrow> bool) \<Rightarrow>
+  ('h \<Rightarrow> _ \<Rightarrow> llvm_amemory \<Rightarrow> bool) \<Rightarrow>
+  ('i \<Rightarrow> _ \<Rightarrow> llvm_amemory \<Rightarrow> bool) \<Rightarrow>
+  ('j \<Rightarrow> _ \<Rightarrow> llvm_amemory \<Rightarrow> bool) \<Rightarrow>
+  ('k \<Rightarrow> _ \<Rightarrow> llvm_amemory \<Rightarrow> bool) \<Rightarrow>
+  ('l \<Rightarrow> _ \<Rightarrow> llvm_amemory \<Rightarrow> bool) \<Rightarrow>
+  ('m \<Rightarrow> _ \<Rightarrow> llvm_amemory \<Rightarrow> bool) \<Rightarrow>
+  ('n \<Rightarrow> _ \<Rightarrow> llvm_amemory \<Rightarrow> bool) \<Rightarrow>
+  ('o \<Rightarrow> _ \<Rightarrow> llvm_amemory \<Rightarrow> bool) \<Rightarrow>
+  ('p \<Rightarrow> _ \<Rightarrow> llvm_amemory \<Rightarrow> bool) \<Rightarrow>
+  ('a, 'b, 'c, 'd, 'e, 'f, 'g, 'h, 'i, 'j,
+     'k, 'l, 'm, 'n, 'o, 'p) isasat_int \<Rightarrow> _ \<Rightarrow> assn\<close> where
+  \<open>isasat_int_assn a_assn b_assn' c_assn d_assn e_assn f_assn g_assn h_assn i_assn j_assn k_assn l_assn m_assn n_assn o_assn p_assn S T =
+   (case (S, T) of
+  (IsaSAT_int M N D i W ivmtf icount ccach lbd outl heur stats aivdom clss opts arena,
+   IsaSAT_int M' N' D' i' W' ivmtf' icount' ccach' lbd' outl' heur' stats' aivdom' clss' opts' arena')
+     \<Rightarrow>
+ (a_assn M (M') \<and>* b_assn' N (N') \<and>* c_assn D (D')  \<and>* d_assn i (i') \<and>*
+ e_assn W (W') \<and>* f_assn ivmtf (ivmtf') \<and>* g_assn icount (icount')  \<and>* h_assn ccach (ccach') \<and>*
+ i_assn lbd (lbd') \<and>* j_assn outl (outl') \<and>* k_assn heur (heur')  \<and>* l_assn stats (stats') \<and>*
+ m_assn aivdom (aivdom') \<and>* n_assn clss (clss') \<and>* o_assn opts (opts')  \<and>* p_assn arena (arena')))
+  \<close>
+
+definition test where
+  \<open>test M = isasat_int.literals_to_update_wl_heur M\<close>
+
+
+
+definition isasat_bounded_assn :: \<open>_ \<Rightarrow> _ \<Rightarrow> assn\<close> where
+\<open>isasat_bounded_assn = isasat_int_assn
+  trail_pol_fast_assn  arena_fast_assn
+  conflict_option_rel_assn
+  sint64_nat_assn
+  watchlist_fast_assn
+  vmtf_remove_assn
+  uint32_nat_assn
+  cach_refinement_l_assn
+  lbd_assn
+  out_learned_assn
+  stats_assn
+  heuristic_assn
+  aivdom_assn
+  lcount_assn
+  opts_assn  arena_fast_assn\<close>
+
+lemma [sepref_fr_rules]: \<open>(Mreturn o isasat_int.literals_to_update_wl_heur, RETURN o isasat_int.literals_to_update_wl_heur) \<in> isasat_bounded_assn\<^sup>k \<rightarrow>\<^sub>a sint64_nat_assn\<close>
+  supply [split] =  isasat_int.splits
+  unfolding isasat_bounded_assn_def
+  apply sepref_to_hoare
+  apply (vcg')
+  done
+sepref_def test_impl
+  is \<open>RETURN o test\<close>
+  :: \<open>isasat_bounded_assn\<^sup>k \<rightarrow>\<^sub>a sint64_nat_assn\<close>
+  unfolding test_def
+  by sepref
+export_llvm test_impl
+
+
+locale isasat_state_ops =
+  fixes
+    a_assn :: \<open>'a \<Rightarrow> 'xa \<Rightarrow> assn\<close> and
+    b_assn :: \<open>'b \<Rightarrow> 'xb \<Rightarrow> assn\<close> and
+    c_assn :: \<open>'c \<Rightarrow> 'xc \<Rightarrow> assn\<close> and
+    d_assn :: \<open>'d \<Rightarrow> 'xd \<Rightarrow> assn\<close> and
+    e_assn :: \<open>'e \<Rightarrow> 'xe \<Rightarrow> assn\<close> and
+    f_assn :: \<open>'f \<Rightarrow> 'xf \<Rightarrow> assn\<close> and
+    g_assn :: \<open>'g \<Rightarrow> 'xg \<Rightarrow> assn\<close> and
+    h_assn :: \<open>'h \<Rightarrow> 'xh \<Rightarrow> assn\<close> and
+    i_assn :: \<open>'i \<Rightarrow> 'xi \<Rightarrow> assn\<close> and
+    j_assn :: \<open>'j \<Rightarrow> 'xj \<Rightarrow> assn\<close> and
+    k_assn :: \<open>'k \<Rightarrow> 'xk \<Rightarrow> assn\<close> and
+    l_assn :: \<open>'l \<Rightarrow> 'xl \<Rightarrow> assn\<close> and
+    m_assn :: \<open>'m \<Rightarrow> 'xm \<Rightarrow> assn\<close> and
+    n_assn :: \<open>'n \<Rightarrow> 'xn \<Rightarrow> assn\<close> and
+    o_assn :: \<open>'o \<Rightarrow> 'xo \<Rightarrow> assn\<close> and
+    p_assn :: \<open>'p \<Rightarrow> 'xp \<Rightarrow> assn\<close> and
+    a_default :: 'a and
+    a :: \<open>unit \<Rightarrow> 'xa llM\<close> and
+    d_default :: 'd and
+    d :: \<open>unit \<Rightarrow> 'xd llM\<close>
+begin
+
+definition isasat_assn :: \<open>_ \<Rightarrow> _ \<Rightarrow> assn\<close> where
+\<open>isasat_assn = isasat_int_assn
+  a_assn b_assn c_assn d_assn
+  e_assn f_assn g_assn h_assn
+  i_assn j_assn k_assn l_assn
+  m_assn n_assn o_assn p_assn\<close>
+
+definition remove_literals_to_update_wl_heur :: \<open>('a, 'b, 'c, 'd, 'e, 'f, 'g, 'h, 'i, 'j,
+     'k, 'l, 'm, 'n, 'o, 'p) isasat_int \<Rightarrow> _ \<times> ('a, 'b, 'c, 'd, 'e, 'f, 'g, 'h, 'i, 'j,
+     'k, 'l, 'm, 'n, 'o, 'p) isasat_int\<close> where
+  \<open>remove_literals_to_update_wl_heur isasat_int = (case isasat_int of IsaSAT_int x1 x2 x3 x4 x5 x6 x7 x8 x9 x10 x11 x12 x13 x14 x15 x16 \<Rightarrow>
+      (x4, IsaSAT_int x1 x2 x3 d_default x5 x6 x7 x8 x9 x10 x11 x12 x13 x14 x15 x16))\<close>
+
+
+definition remove_literals_to_update_wl_heur_int :: \<open>('xa, 'xb, 'xc, 'xd, 'xe, 'xf, 'xg, 'xh, 'xi, 'xj,
+     'xk, 'xl, 'xm, 'xn, 'xo, 'xp) isasat_int \<Rightarrow> ('xd \<times> ('xa, 'xb, 'xc, 'xd, 'xe, 'xf, 'xg, 'xh, 'xi, 'xj,
+     'xk, 'xl, 'xm, 'xn, 'xo, 'xp) isasat_int, _) M\<close> where
+  \<open>remove_literals_to_update_wl_heur_int isasat_int =
+    (case isasat_int of IsaSAT_int x1 x2 x3 x4 x5 x6 x7 x8 x9 x10 x11 x12 x13 x14 x15 x16 \<Rightarrow>
+     doM{
+    d' \<leftarrow> d ();
+    S \<leftarrow> Mreturn (IsaSAT_int x1 x2 x3 d' x5 x6 x7 x8 x9 x10 x11 x12 x13 x14 x15 x16);
+    Mreturn (x4, S)
+  })\<close>
+end
+
+
+
+locale isasat_state =
+  isasat_state_ops a_assn b_assn c_assn d_assn e_assn
+  f_assn g_assn h_assn i_assn j_assn
+  k_assn l_assn m_assn n_assn o_assn p_assn
+  a_default a
+  d_default d
+  for
+    a_assn :: \<open>'a \<Rightarrow> 'xa \<Rightarrow> assn\<close> and
+    b_assn :: \<open>'b \<Rightarrow> 'xb \<Rightarrow> assn\<close> and
+    c_assn :: \<open>'c \<Rightarrow> 'xc \<Rightarrow> assn\<close> and
+    d_assn :: \<open>'d \<Rightarrow> 'xd \<Rightarrow> assn\<close> and
+    e_assn :: \<open>'e \<Rightarrow> 'xe \<Rightarrow> assn\<close> and
+    f_assn :: \<open>'f \<Rightarrow> 'xf \<Rightarrow> assn\<close> and
+    g_assn :: \<open>'g \<Rightarrow> 'xg \<Rightarrow> assn\<close> and
+    h_assn :: \<open>'h \<Rightarrow> 'xh \<Rightarrow> assn\<close> and
+    i_assn :: \<open>'i \<Rightarrow> 'xi \<Rightarrow> assn\<close> and
+    j_assn :: \<open>'j \<Rightarrow> 'xj \<Rightarrow> assn\<close> and
+    k_assn :: \<open>'k \<Rightarrow> 'xk \<Rightarrow> assn\<close> and
+    l_assn :: \<open>'l \<Rightarrow> 'xl \<Rightarrow> assn\<close> and
+    m_assn :: \<open>'m \<Rightarrow> 'xm \<Rightarrow> assn\<close> and
+    n_assn :: \<open>'n \<Rightarrow> 'xn \<Rightarrow> assn\<close> and
+    o_assn :: \<open>'o \<Rightarrow> 'xo \<Rightarrow> assn\<close> and
+    p_assn :: \<open>'p \<Rightarrow> 'xp \<Rightarrow> assn\<close> and
+    a_default :: 'a and
+    a :: \<open>unit \<Rightarrow> 'xa llM\<close> and
+    d_default :: 'd and
+    d :: \<open>unit \<Rightarrow> 'xd llM\<close> +
+  assumes
+    a: \<open>(a, uncurry0 (RETURN a_default)) \<in> unit_assn\<^sup>k \<rightarrow>\<^sub>a a_assn\<close> and
+    d: \<open>(d, uncurry0 (RETURN d_default)) \<in> unit_assn\<^sup>k \<rightarrow>\<^sub>a d_assn\<close>
+begin
+
+lemmas [sepref_fr_rules] = d
+
+lemma ex_isasat_int_iff: "(\<exists>b :: (_,_,_,_,_,_,_,_,_,_,_,_,_,_,_,_)isasat_int. P b) \<longleftrightarrow>
+  (\<exists>a b  c d e f g h i j k l m n ko p. P (IsaSAT_int a b  c d e f g h i j k l m n ko p))"
+  apply auto
+    apply (case_tac b)
+  by force
+lemma remove_literals_to_update_wl_heur_int:
+  \<open>(remove_literals_to_update_wl_heur_int, RETURN o remove_literals_to_update_wl_heur) \<in> isasat_assn\<^sup>d \<rightarrow>\<^sub>a d_assn \<times>\<^sub>a isasat_assn\<close>
+  unfolding remove_literals_to_update_wl_heur_int_def remove_literals_to_update_wl_heur_def isasat_assn_def
+  supply [split] =  isasat_int.splits
+  apply sepref_to_hoare
+  apply (case_tac x)
+  apply vcg
+  unfolding wpa_return
+  apply auto
+  apply (subst (asm)(2) sep_algebra_class.sep_conj_empty'[symmetric])
+  apply (rule apply_htriple_rule)
+  apply assumption
+  apply (rule d[to_hnr, simplified, unfolded hn_refine_def, rule_format])
+  apply auto[]
+  apply (rule POSTCONDI)
+  apply (rule STATE_monoI)
+  apply assumption
+  apply (auto simp: Exists_eq_simp ex_isasat_int_iff)
+  subgoal premises p for x1 x2 x3 x4 x5 x6 x7 x8 x9 x10 x11 x12 x13 x14 x15 x16 x1a x2a x3a x4a x5a x6a x7a x8a x9a x10a x11a x12a x13a x14a x15a x16a asf s s' r
+    by (smt (z3) entails_def entails_eq_iff pure_true_conv sep_conj_aci(4) sep_conj_aci(5) sep_conj_left_commute)
+  done
+end
+definition extract_literals_to_update_wl_heur where
+  \<open>extract_literals_to_update_wl_heur = isasat_state_ops.remove_literals_to_update_wl_heur 0\<close>
+
+definition bottom_trail :: trail_pol where
+  \<open>bottom_trail = do {
+     let M0 = [] in
+     let cs = [] in
+     let M = replicate 0 UNSET in
+     let M' = replicate 0 0 in
+     let M'' = replicate 0 1 in
+    ((M0, M, M', M'', 0, cs))
+}\<close>
+
+sepref_def bottom_trail_code
+  is \<open>uncurry0 (RETURN bottom_trail)\<close>
+  :: \<open>unit_assn\<^sup>k \<rightarrow>\<^sub>a trail_pol_fast_assn\<close>
+  unfolding bottom_trail_def trail_pol_fast_assn_def
+  apply (rewrite in \<open>let _ = \<hole> in _\<close> annotate_assn[where A=\<open>arl64_assn unat_lit_assn\<close>])
+  apply (rewrite in \<open>let _ = \<hole> in _\<close> al_fold_custom_empty[where 'l=64])
+  apply (rewrite in \<open>let _ = _; _ = \<hole> in _\<close> al_fold_custom_empty[where 'l=64])
+  apply (rewrite in \<open>let _ = _; _ = \<hole> in _\<close> annotate_assn[where A=\<open>arl64_assn uint32_nat_assn\<close>])
+
+  apply (rewrite in \<open>let _ = _;_ = \<hole> in _\<close> annotate_assn[where A=\<open>larray64_assn (tri_bool_assn)\<close>])
+  apply (rewrite in \<open>let _ = _;_ = _;_ = \<hole> in _\<close> annotate_assn[where A=\<open>larray64_assn uint32_nat_assn\<close>])
+  apply (rewrite in \<open>let _ = _ in _\<close> larray_fold_custom_replicate)
+  apply (rewrite in \<open>let _ = _ in _\<close> larray_fold_custom_replicate)
+  apply (rewrite in \<open>let _ = _ in _\<close> larray_fold_custom_replicate)
+  apply (rewrite at \<open>(_, \<hole>, _)\<close> unat_const_fold[where 'a=32])
+  apply (rewrite at \<open>(op_larray_custom_replicate _ \<hole>)\<close> unat_const_fold[where 'a=32])
+  apply (annot_snat_const \<open>TYPE(64)\<close>)
+  supply [[goals_limit = 1]]
+  by sepref
+
+
+global_interpretation isasat_state where
+  a_assn = trail_pol_fast_assn and
+  b_assn = arena_fast_assn and
+  c_assn = conflict_option_rel_assn and
+  d_assn = sint64_nat_assn and
+  e_assn = watchlist_fast_assn and
+  f_assn = vmtf_remove_assn and
+  g_assn = uint32_nat_assn and
+  h_assn = cach_refinement_l_assn and
+  i_assn = lbd_assn and
+  j_assn = out_learned_assn and
+  k_assn = stats_assn and
+  l_assn = heuristic_assn and
+  m_assn = aivdom_assn and
+  n_assn = lcount_assn and
+  o_assn = opts_assn and
+  p_assn = arena_fast_assn and
+  a_default = bottom_trail and
+  a = \<open>uncurry0 bottom_trail_code\<close> and
+  d = \<open>uncurry0 (Mreturn 0)\<close> and
+  d_default = \<open>0\<close>
+  rewrites
+    \<open>isasat_assn \<equiv> isasat_bounded_assn\<close> and
+    \<open>remove_literals_to_update_wl_heur \<equiv> extract_literals_to_update_wl_heur\<close>
+  apply unfold_locales
+  subgoal by (rule bottom_trail_code.refine)
+  subgoal
+    by (sepref_to_hoare, vcg)
+     (auto simp: snat_rel_def snat.rel_def br_def Exists_eq_simp snat_invar_0 pure_true_conv entails_def ENTAILS_def)
+  subgoal
+    unfolding isasat_bounded_assn_def isasat_state_ops.isasat_assn_def
+    .
+  subgoal
+    unfolding extract_literals_to_update_wl_heur_def
+      .
+  done
+
+lemmas [sepref_fr_rules] = remove_literals_to_update_wl_heur_int
+  thm remove_literals_to_update_wl_heur_int
+declare remove_literals_to_update_wl_heur_int_def[llvm_inline]
+
+
+definition test2 where
+  \<open>test2 M = do {a \<leftarrow> RETURN (extract_literals_to_update_wl_heur M);  (i, M) \<leftarrow> RETURN a; ASSERT (i+1 < 100); RETURN (i+1, M)}\<close>
+sepref_register extract_literals_to_update_wl_heur
+sepref_def test_impl3
+  is \<open>test2\<close>
+  :: \<open>isasat_bounded_assn\<^sup>d \<rightarrow>\<^sub>a sint64_nat_assn \<times>\<^sub>a isasat_bounded_assn\<close>
+  supply [[goals_limit=1]]
+  unfolding test2_def
+  apply (annot_snat_const \<open>TYPE(64)\<close>)
+  by sepref
+
+   term ll_bpto
+  lemma [llvm_pre_simp]: \<open>uncurry0 f () = f\<close>
+     by auto
+
+  thm remove_literals_to_update_wl_heur_int_def
+export_llvm test_impl3
+
+  sepref_def test
+    is \<open>RETURN o remove_literals_to_update_wl_heur\<close>
+    :: \<open>isasat_assn\<^sup>d \<rightarrow>\<^sub>a d_assn \<times>\<^sub>a isasat_assn\<close>
+    unfolding remove_literals_to_update_wl_heur_def
+    apply sepref
+term isasat_bounded_assn
+lemma [sepref_fr_rules]:
+  \<open>(remove_literals_to_update_wl_heur_int, RETURN o remove_literals_to_update_wl_heur_int) \<in> isasat_assn\<^sup>d \<rightarrow>\<^sub>a arena_fast_assn \<times>\<^sub>a isasat_id_assn\<close>
+  term aa
+  term a
+  supply [split] =  isasat_int.splits
+  unfolding remove_literals_to_update_wl_heur_int_def
+  apply sepref_to_hoare
+  apply (case_tac x)
+  apply vcg
+  done
+      find_theorems op_al_empty
+find_theorems name:empty name:al
+definition remove_literals_to_update_wl_heur where \<open>remove_literals_to_update_wl_heur = remove_literals_to_update_wl_heur_int\<close>
+
+sepref_register remove_literals_to_update_wl_heur_int remove_literals_to_update_wl_heur
+sepref_def remove_literals_to_update_wl_heur_impl
+  is \<open>RETURN o remove_literals_to_update_wl_heur\<close>
+  :: \<open>id_assn\<^sup>d \<rightarrow>\<^sub>a word64_assn \<times>\<^sub>a id_assn\<close>
+  unfolding remove_literals_to_update_wl_heur_def
+  by sepref
+
+
+declare remove_literals_to_update_wl_heur_int_def[llvm_inline]
+export_llvm test_impl3
+term ll_pto
+find_theorems "_ :: isasat_int \<Rightarrow> assn"
 
 type_synonym twl_st_wll_trail_fast =
   \<open>trail_pol_fast_assn \<times> arena_assn \<times> option_lookup_clause_assn \<times>
